MAJOR: use finmap, occurs

src/exp/core.lean
@@ -1,84 +1,129 @@
+import data.fresh
 import data.finset
+import occurs
 
 namespace tts ------------------------------------------------------------------
 
+open occurs
+
 -- Grammar of expressions.
 inductive exp (V : Type) : Type
-  | varb {} : ℕ → exp          -- bound variable
-  | varf    : V → exp          -- free variable
-  | app     : exp → exp → exp  -- function application
-  | lam     : exp → exp        -- lambda-abstraction
-  | let_    : exp → exp → exp  -- let-abstraction
+  | var  : occurs → tagged V → exp -- variable, bound or free
+  | app  : exp → exp → exp         -- function application
+  | lam  : V → exp → exp           -- lambda-abstraction
+  | let_ : V → exp → exp → exp     -- let-abstraction
 
 variables {V : Type} -- Type of variable names
 
 namespace exp ------------------------------------------------------------------
 
--- Open an expression (last parameter) with an expression (eb) for a bound
--- variable.
 protected
-def open.rec (e : exp V) : ℕ → exp V → exp V
-  | k (varb i)     := if k = i then e else varb i
-  | k (varf x)     := varf x
-  | k (app ef ea)  := app (open.rec k ef) (open.rec k ea)
-  | k (lam eb)     := lam (open.rec (k + 1) eb)
-  | k (let_ ed eb) := let_ (open.rec k ed) (open.rec (k + 1) eb)
+def repr [has_repr V] : exp V → string
+  | (var bound x)  := _root_.repr x.tag ++ "⟨" ++ _root_.repr x.val ++ "⟩"
+  | (var free x)   := _root_.repr x
+  | (app ef ea)    := "(" ++ ef.repr ++ ") (" ++ ea.repr ++ ")"
+  | (lam v eb)     := "λ " ++ _root_.repr v ++ " . " ++ eb.repr
+  | (let_ v ed eb) := "let " ++ _root_.repr v ++ " = " ++ ed.repr ++ " in " ++ eb.repr
+
+instance [has_repr V] : has_repr (exp V) :=
+⟨exp.repr⟩
+
+-- Open an expression (last parameter) with an expression (e) for a bound
+-- variable.
+def open_exp (e : exp V) : ℕ → exp V → exp V
+  | k (var bound x)  := if k = x.tag then e else var bound x
+  | _ (var free x)   := var free x
+  | k (app ef ea)    := app (open_exp k ef) (open_exp k ea)
+  | k (lam v eb)     := lam v (open_exp k.succ eb)
+  | k (let_ v ed eb) := let_ v (open_exp k ed) (open_exp k.succ eb)
+
+@[simp]
+theorem open_exp_var_bound_eq {k} {x : tagged V} {e : exp V} (h : k = x.tag)
+: open_exp e k (var bound x) = e :=
+  by simp [open_exp, h]
+
+@[simp]
+theorem open_exp_var_bound_ne {k} {x : tagged V} {e : exp V} (h : k ≠ x.tag)
+: open_exp e k (var bound x) = var bound x :=
+  by simp [open_exp, h]
+
+@[simp]
+theorem open_exp_var_free {k} {x : tagged V} {e : exp V}
+: open_exp e k (var free x) = var free x :=
+  rfl
+
+@[simp]
+theorem open_exp_app {k} {e ef ea : exp V}
+: open_exp e k (app ef ea) = app (open_exp e k ef) (open_exp e k ea) :=
+  rfl
+
+@[simp]
+theorem open_exp_lam {k v} {e eb : exp V}
+: open_exp e k (lam v eb) = lam v (open_exp e k.succ eb) :=
+  rfl
+
+@[simp]
+theorem open_exp_let_ {k v} {e ed eb : exp V}
+: open_exp e k (let_ v ed eb) = let_ v (open_exp e k ed) (open_exp e k.succ eb) :=
+  rfl
+
+-- Open an expression with an expression `e` for the last bound variable (0).
+def open_exp₀ (e : exp V) : exp V → exp V :=
+  open_exp e 0
+
+-- Open an expression with a free variable `x` for the last bound variable.
+def open_var (x : tagged V) : exp V → exp V :=
+  open_exp₀ (var free x)
 
 variables [decidable_eq V]
 
+-- Open an expression with a variable of the name `v` fresh from the variable
+-- set `L` for the last bound variable.
+def open_fresh (v : V) (L : finset (tagged V)) : exp V → exp V :=
+  open_var $ (fresh.tagged v).gen L
+
 -- Get the free variables of an expression
-def fv : exp V → finset V
-  | (varb i)     := ∅
-  | (varf x)     := {x}
-  | (app ef ea)  := fv ef ∪ fv ea
-  | (lam eb)     := fv eb
-  | (let_ ed eb) := fv ed ∪ fv eb
+def fv : exp V → finset (tagged V)
+  | (var bound _)  := ∅
+  | (var free x)   := {x}
+  | (app ef ea)    := fv ef ∪ fv ea
+  | (lam _ eb)     := fv eb
+  | (let_ _ ed eb) := fv ed ∪ fv eb
 
 -- Substitute a free variable for an expression in an expression
-def subst (x : V) (e : exp V) : exp V → exp V
-  | (varb i)     := varb i
-  | (varf y)     := if x = y then e else varf y
-  | (app ef ea)  := app (subst ef) (subst ea)
-  | (lam eb)     := lam (subst eb)
-  | (let_ ed eb) := let_ (subst ed) (subst eb)
+def subst (x : tagged V) (e : exp V) : exp V → exp V
+  | (var bound y)  := var bound y
+  | (var free y)   := if x = y then e else var free y
+  | (app ef ea)    := app (subst ef) (subst ea)
+  | (lam v eb)     := lam v (subst eb)
+  | (let_ v ed eb) := let_ v (subst ed) (subst eb)
 
 end /- namespace -/ exp --------------------------------------------------------
 
--- Open an expression with an expression (eb) for the last bound variable (0).
--- Note: This definition is defined outside the `exp` namespace because it
--- conflicts with the keyword `open` if declared without the `exp`. prefix.
-protected
-def exp.open (eb : exp V) : exp V → exp V :=
-  exp.open.rec eb 0
-
 namespace exp ------------------------------------------------------------------
+variables [decidable_eq V]
 
--- Open an expression with a free variable (x) for the last bound variable (0).
-def open_var (x : V) : exp V → exp V :=
-  exp.open (varf x)
-
--- Property of a locally-closed expression
 inductive lc : exp V → Prop
-  | varf : Π (x : V),                                                                          lc (varf x)
-  | app  : Π                {ef ea : exp V}, lc ef → lc ea →                                   lc (app ef ea)
-  | lam  : Π {L : finset V} {eb : exp V},            (∀ {x : V}, x ∉ L → lc (open_var x eb)) → lc (lam eb)
-  | let_ : Π {L : finset V} {ed eb : exp V}, lc ed → (∀ {x : V}, x ∉ L → lc (open_var x eb)) → lc (let_ ed eb)
+  | var  : Π x,                                                                                                    lc (var free x)
+  | app  : Π                {ef ea : exp V},              lc ef → lc ea →                                          lc (app ef ea)
+  | lam  : Π {v} (L : finset (tagged V)) {eb : exp V},            (∀ {x : tagged V}, x ∉ L → lc (open_var x eb)) → lc (lam v eb)
+  | let_ : Π {v} (L : finset (tagged V)) {ed eb : exp V}, lc ed → (∀ {x : tagged V}, x ∉ L → lc (open_var x eb)) → lc (let_ v ed eb)
 
 -- Locally-closed body of a lambda- or let-expression
-def lc_body (eb : exp V) : Prop :=
-  ∃ (L : finset V), ∀ {x : V}, x ∉ L → (open_var x eb).lc
+def lc_body (e : exp V) : Prop :=
+  ∃ (L : finset (tagged V)), ∀ {x : tagged V}, x ∉ L → lc (open_var x e)
 
 -- Grammar of values
 inductive value : exp V → Prop
-  | lam  : Π {e : exp V}, e.lc_body → value (lam e)
+  | lam : Π {v} {e : exp V}, lc_body e → value (lam v e)
 
 -- Reduction rules
 inductive red : exp V → exp V → Prop
-  | app₁  : Π {ef ef' ea : exp V}, red ef ef' → ea.lc      → red (app ef ea)       (app ef' ea)
-  | app₂  : Π {ef ea ea' : exp V}, ef.value   → red ea ea' → red (app ef ea)       (app ef ea')
-  | lam   : Π {eb ea : exp V},     eb.lc_body → ea.value   → red (app (lam eb) ea) (exp.open ea eb)
-  | let₁  : Π {ed ed' eb : exp V}, red ed ed' → eb.lc_body → red (let_ ed eb)      (let_ ed' eb)
-  | let₂  : Π {ed eb : exp V},     ed.value   → eb.lc_body → red (let_ ed eb)      (exp.open ed eb)
+  | app₁  : Π {ef ef' ea : exp V},         red ef ef' → ea.lc      → red (app ef ea)         (app ef' ea)
+  | app₂  : Π {ef ea ea' : exp V},         value ef   → red ea ea' → red (app ef ea)         (app ef ea')
+  | lam   : Π {v : V} {eb ea : exp V},     lc_body eb → value ea   → red (app (lam v eb) ea) (open_exp₀ ea eb)
+  | let₁  : Π {v : V} {ed ed' eb : exp V}, red ed ed' → lc_body eb → red (let_ v ed eb)      (let_ v ed' eb)
+  | let₂  : Π {v : V} {ed eb : exp V},     value ed   → lc_body eb → red (let_ v ed eb)      (open_exp₀ ed eb)
 
 end /- namespace -/ exp --------------------------------------------------------
 end /- namespace -/ tts --------------------------------------------------------
