src/sch/core.lean
@@ -1,5 +1,5 @@
+import data.fresh
 import typ.core
-import data.finset.disjoint_list
 
 namespace tts ------------------------------------------------------------------
 
@@ -16,43 +16,52 @@ variables {V : Type} -- Type of variable names
 namespace sch ------------------------------------------------------------------
 variables [_root_.decidable_eq V]
 
+theorem eq_of_veq : ∀ {s₁ s₂ : sch V}, s₁.arity = s₂.arity → s₁.type = s₂.type → s₁ = s₂
+| ⟨a₁, t₁⟩ ⟨a₂, t₂⟩ ha ht := by congr; solve_by_elim
+
 -- Get the free variables of a scheme.
-def fv (s : sch V) : finset V :=
-  s.type.fv
+def fv (s : sch V) : finset (tagged V) :=
+  typ.fv s.type
+
+@[simp]
+theorem fv_mk {a : ℕ} {t : typ V} : fv (mk a t) = typ.fv t :=
+  rfl
 
 -- Substitute a free variable for a type in a scheme
-def subst (x : V) (t : typ V) (s : sch V) : sch V :=
+def subst (x : tagged V) (t : typ V) (s : sch V) : sch V :=
   ⟨s.arity, typ.subst x t s.type⟩
 
+@[simp]
+theorem subst_mk {a : ℕ} {x : tagged V} {tx t : typ V} : subst x tx (mk a t) = mk a (typ.subst x tx t) :=
+  rfl
+
 -- Substitute a list of free variables for a list of types in a scheme
-def subst_list (xs : list V) (ts : list (typ V)) (s : sch V) : sch V :=
+def subst_list (xs : list (tagged V)) (ts : list (typ V)) (s : sch V) : sch V :=
   ⟨s.arity, typ.subst_list xs ts s.type⟩
 
-end /- namespace -/ sch --------------------------------------------------------
+@[simp]
+theorem subst_list_mk {a : ℕ} {xs : list (tagged V)} {ts : list (typ V)} {t : typ V} : subst_list xs ts (mk a t) = mk a (typ.subst_list xs ts t) :=
+  rfl
 
--- Open a type scheme with a list of expressions for bound variables.
--- Note: This definition is defined outside the `sch` namespace because it
--- conflicts with the keyword `open` if declared without the `sch`. prefix.
-protected
-def sch.open (ts : list (typ V)) (s : sch V) : typ V :=
-  s.type.open ts
+-- Open a type scheme with a list of types for bound variables.
+def open_typs (ts : list (typ V)) (s : sch V) : typ V :=
+  typ.open_typs ts s.type
 
-namespace sch ------------------------------------------------------------------
+@[simp]
+theorem open_typs_mk {ts : list (typ V)} {a : ℕ} {t : typ V} : open_typs ts (mk a t) = typ.open_typs ts t :=
+  rfl
 
 -- Open a type scheme with a list of free variables for bound variables.
-def open_vars (xs : list V) (s : sch V) : typ V :=
-  s.type.open_vars xs
+def open_vars (xs : list (tagged V)) (s : sch V) : typ V :=
+  typ.open_vars xs s.type
 
-variables [_root_.decidable_eq V]
+@[simp]
+theorem open_vars_mk {xs : list (tagged V)} {a : ℕ} {t : typ V} : open_vars xs (mk a t) = typ.open_vars xs t :=
+  rfl
 
--- Property of a well-formed scheme.
-def well_formed (s : sch V) : Prop :=
-  ∃ (L : finset V)
-  , ∀ {xs : list V}
-  , xs.nodup
-  → xs.length = s.arity
-  → finset.disjoint_list xs L
-  → typ.lc (sch.open_vars xs s)
+-- A scheme is locally-closed if its body is locally closed.
+def lc (s : sch V) : Prop :=
+  typ.lc_body s.arity s.type
 
 end /- namespace -/ sch --------------------------------------------------------
 end /- namespace -/ tts --------------------------------------------------------
