src/env.lean
@@ -1,0 +1,33 @@
+import data.finmap
+import sch
+
+namespace tts ------------------------------------------------------------------
+
+/-- Binding type -/
+abbreviation bty (V : Type) (x : tagged V) : Type :=
+sch V
+
+/-- A (non-dependent) pair of a variable and a type scheme -/
+abbreviation binding (V : Type) : Type :=
+sigma (bty V)
+
+/-- Construct a binding -/
+abbreviation binding.mk {V : Type} : tagged V → sch V → binding V :=
+sigma.mk
+
+/- Notation for a binding -/
+infix ` :~ `:80 := binding.mk
+
+/-- Free variables of a binding -/
+abbreviation binding.fv {V : Type} [decidable_eq V] (b : binding V) : finset (tagged V) :=
+sch.fv b.2
+
+/-- Environment mapping variables to bindings -/
+abbreviation env (V : Type) : Type :=
+finmap (tagged V) (bty V)
+
+/-- Domain of an environment -/
+abbreviation dom {V : Type} (Γ : env V) : finset (tagged V) :=
+finmap.keys Γ
+
+end /- namespace -/ tts --------------------------------------------------------
