src/exp/open.lean
@@ -1,54 +1,58 @@
-import .core
-import data.finset.fresh
+import .lc
 
 namespace tts ------------------------------------------------------------------
 namespace exp ------------------------------------------------------------------
 variables {V : Type} -- Type of variable names
 
+open occurs
+
 -- Properties of open
 
 lemma open_lc.core {e₁ e₂ e₃ : exp V} {k₂ k₃ : ℕ} (p : k₂ ≠ k₃)
-: open.rec e₂ k₂ (open.rec e₃ k₃ e₁) = open.rec e₃ k₃ e₁ → open.rec e₂ k₂ e₁ = e₁ :=
+: open_exp e₂ k₂ (open_exp e₃ k₃ e₁) = open_exp e₃ k₃ e₁ → open_exp e₂ k₂ e₁ = e₁ :=
   begin
-    induction e₁ generalizing e₂ e₃ k₂ k₃; repeat {rw open.rec},
-    case exp.varb : i {
-      by_cases h : k₃ = i,
-      {/- h : k₃ = i -/ induction h, rw [if_pos (eq.refl k₃), if_neg p], intro, refl},
-      {/- h : k₃ ≠ i -/ rw [if_neg h, open.rec], exact id}
+    induction e₁ generalizing e₂ e₃ k₂ k₃; repeat {rw open_exp},
+    case exp.var : o x {
+      cases o,
+      case occurs.bound {
+        cases x with _ i,
+        by_cases h : k₃ = i,
+        { induction h, simp [p] },
+        { simp [h] }
+      },
+      case occurs.free { exact id },
     },
-    case exp.varf : x {
-      exact id
-    },
-    case exp.app : ef ea rf ra {
+    case exp.app : ef ea ihf iha {
       intro h,
       injection h with hf ha,
-      conv {to_lhs, rw [rf p hf, ra p ha]}
+      conv {to_lhs, rw [ihf p hf, iha p ha]}
     },
-    case exp.lam : eb rb {
+    case exp.lam : v eb rb {
       intro h,
-      injection h with hb,
+      injection h with _ hb,
       conv {to_lhs, rw rb (mt nat.succ.inj p) hb}
     },
-    case exp.let_ : ed eb rd rb {
+    case exp.let_ : v ed eb rd rb {
       intro h,
-      injection h with hd hb,
+      injection h with _ hd hb,
       conv {to_lhs, rw [rd p hd, rb (mt nat.succ.inj p) hb]}
     }
   end
 
-variables [finset.has_fresh V]
+variables [decidable_eq V]
 
-lemma open_lc.rec {e₁ e₂ : exp V} {k : ℕ} (l : lc e₁) : open.rec e₂ k e₁ = e₁ :=
+@[simp]
+lemma open_exp_of_lc {e₁ e₂ : exp V} {k : ℕ} (l : lc e₁) : open_exp e₂ k e₁ = e₁ :=
   begin
-    induction l generalizing e₂ k; rw open.rec,
+    induction l generalizing e₂ k; rw open_exp,
     case lc.app : ef ea lf la rf ra {
       rw [rf, ra]
     },
-    case lc.lam : L eb Fb rb {
-      rw open_lc.core (nat.succ_ne_zero k) (rb (finset.fresh_not_mem L))
+    case lc.lam : v L eb lb rb {
+      rw open_lc.core k.succ_ne_zero (rb ((fresh.tagged v).gen_not_mem L))
     },
-    case lc.let_ : L ed eb ld Fb rd rb {
-      rw [rd, open_lc.core (nat.succ_ne_zero k) (rb (finset.fresh_not_mem L))]
+    case lc.let_ : v L ed eb ld Fb rd rb {
+      rw [rd, open_lc.core k.succ_ne_zero (rb ((fresh.tagged v).gen_not_mem L))]
     }
   end
 
