src/occurs.lean
@@ -1,0 +1,29 @@
+import data.equiv.basic
+
+namespace tts ------------------------------------------------------------------
+
+/-- An enumeration of the states in which a variable can occur with respect to
+bindings. `occurs` is isomorphic to `bool` but more descriptive in naming. -/
+@[derive decidable_eq]
+inductive occurs : Type
+| bound : occurs -- Referenced by a binding
+| free  : occurs -- Not referenced by any binding (unbound)
+
+namespace occurs ---------------------------------------------------------------
+
+@[simp] def is_free : occurs → bool
+| bound := ff
+| free  := tt
+
+@[simp] def of_free : bool → occurs
+| ff := bound
+| tt := free
+
+def equiv_bool : occurs ≃ bool :=
+⟨is_free, of_free, λ o, by cases o; simp, λ b, by cases b; simp⟩
+
+@[reducible] instance : has_coe occurs bool :=
+⟨is_free⟩
+
+end /- namespace -/ occurs -----------------------------------------------------
+end /- namespace -/ tts --------------------------------------------------------
