src/sch/subst.lean
@@ -1,13 +1,12 @@
 import .core
 import typ
-import data.finset.fresh
 
 namespace tts ------------------------------------------------------------------
 namespace sch ------------------------------------------------------------------
 variables {n : ℕ} -- Natural numbers
 variables {V : Type} -- Type of variable names
-variables {x x₁ x₂ : V} -- Variable names
-variables {xs : list V} -- List of variable names
+variables {x x₁ x₂ : tagged V} -- Variables
+variables {xs : list (tagged V)} -- List of variable names
 variables {t t₁ t₂ : typ V} -- Types
 variables {ts : list (typ V)} -- Lists of types
 variables {s : sch V} -- Schemes
@@ -15,50 +14,55 @@ variables {s : sch V} -- Schemes
 variables [_root_.decidable_eq V]
 
 -- Substitution with a fresh name is the identity
+@[simp]
 theorem subst_fresh (h : x ∉ fv s) : subst x t s = s :=
-  by cases s; rw [subst, typ.subst_fresh h]
+  eq_of_veq rfl $ typ.subst_fresh h
 
 -- Fold typ.subst into sch.subst
-theorem subst_fold : sch.mk n (typ.subst x t₂ t₁) = subst x t₂ (sch.mk n t₁) :=
+theorem subst_fold : mk n (typ.subst x t₂ t₁) = subst x t₂ (mk n t₁) :=
   rfl
 
 -- Substitution distributes over open
-theorem subst_open (lc_t : typ.lc t)
-: typ.subst x t (sch.open ts s) = sch.open (list.map (typ.subst x t) ts) (subst x t s) :=
-  by cases s; unfold sch.open; rw [subst, typ.subst_open lc_t]
+theorem subst_open (l : typ.lc t)
+: typ.subst x t (open_typs ts s) = open_typs (list.map (typ.subst x t) ts) (subst x t s) :=
+  by cases s; simp [typ.subst_open l]
 
 -- Substitution distributes over open_vars
-theorem subst_open_vars (p : x ∉ xs) (lc_t : typ.lc t)
+theorem subst_open_vars (h : x ∉ xs) (l : typ.lc t)
 : open_vars xs (subst x t s) = typ.subst x t (open_vars xs s) :=
-  by cases s; unfold open_vars; rw [subst, typ.subst_open_vars p lc_t]
+  by cases s; simp [typ.subst_open_vars h l]
 
 @[simp]
 theorem subst_arity : (subst x t s).arity = s.arity :=
   by unfold subst
 
+@[simp]
+theorem subst_type : (subst x t s).type = typ.subst x t s.type :=
+  by unfold subst
+
 -- A scheme substituted with a type is well-formed if the scheme is well-formed
 -- and the type is locally-closed.
-theorem subst_well_formed (lc_t : typ.lc t) (wf_s : well_formed s)
-: well_formed (subst x t s) :=
+theorem subst_well_formed (lt : typ.lc t) (ls : lc s) : lc (subst x t s) :=
   begin
-    cases wf_s with L wf,
-    existsi L ∪ {x},
-    intros xs nd ln dj,
-    simp at dj,
-    rw subst_open_vars dj.2 lc_t,
-    exact typ.subst_lc lc_t (wf nd (by rwa subst_arity at ln) dj.1),
+    cases ls with L ls,
+    existsi insert x L,
+    intros xs d ln_eq F,
+    simp [not_or_distrib] at F,
+    have h₁ : x ∉ xs := λ h, absurd (eq.refl x) (F h).1,
+    have h₂ : ∀ x ∈ xs, x ∉ L := λ _ h, (F h).2,
+    simp [typ.subst_open_vars h₁ lt, typ.subst_lc lt (ls d ln_eq h₂)],
   end
 
 -- Opening up a scheme `s` with `ts` is the same as opening up `s` with fresh
 -- names `xs` and then substituting `xs` for `ts`.
 theorem subst_list_intro
-(nd_xs : xs.nodup)
-(ln_xs_ts : xs.length = ts.length)
-(fr_xs : finset.disjoint_list xs (fv s ∪ typ.fv_list ts))
-(lc_ts : ∀ t ∈ ts, typ.lc t)
-: sch.open ts s = typ.subst_list xs ts (open_vars xs s) :=
-  by unfold sch.open sch.open_vars;
-     exact typ.subst_list_intro nd_xs ln_xs_ts fr_xs lc_ts
+(d : xs.nodup)
+(ln_eq : xs.length = ts.length)
+(F : ∀ x ∈ xs, x ∉ fv s ∪ typ.fv_list ts)
+(l : ∀ t ∈ ts, typ.lc t)
+: open_typs ts s = typ.subst_list xs ts (open_vars xs s) :=
+  by unfold open_typs open_vars;
+     exact typ.subst_list_intro d ln_eq F l
 
 end /- namespace -/ sch --------------------------------------------------------
 end /- namespace -/ tts --------------------------------------------------------
